%include thesis.fmt
%include catch.fmt

%format /# = "/"

\hsdef{\begin{comment}
k,f,c,v,i,on,xs_i,x,ys_i,s,a,ws,c',ms_1,ms_2
vs,xs,y,as,ys,cs,rhs,lhs,g,f_lhd,f_rhd,ks
\end{comment}}
\begin{comment}
\h{#*}\begin{code}
import Prelude hiding (($),(/))
import Data.List

infixr 1  $
infixr 0  ==>
class Implies a where (==>) :: a -> a -> Bool
($) :: (a -> b) -> a -> b

instance Implies Bool
instance Implies (Prop a)

type FuncName = String
type CtorName = String
type VarName = String

freeVars :: Expr -> [String]
body   :: FuncName  -> Expr
args   :: FuncName  -> [VarName]
var    :: VarName   -> Maybe (Expr, Selector)
ctors  :: CtorName  -> [CtorName]
arity :: String -> Int
type Selector  =  (CtorName, Int)
isRec :: Selector -> Bool

precond   :: FuncName -> Prop (Sat VarName)
prePost   :: FuncName -> Constraint -> Prop (Sat VarName)
pre ::  Expr -> Prop (Sat Expr)
reduce    :: Prop (Sat Expr) -> Prop (Sat VarName)
red :: Expr -> Constraint -> Prop (Sat VarName)
substP :: Eq alpha => [(alpha,beta)] -> Prop (Sat alpha) -> Prop (Sat beta)

data Sat alpha = Sat alpha Constraint
instance Eq a => Eq (Sat a)

(-<)  :: alpha -> [CtorName] -> Prop (Sat alpha)
(|>)  :: Selector -> Constraint -> Constraint
(<|)  :: CtorName -> Constraint -> Prop (Sat Int)

data Prop alpha
instance Eq a => Eq (Prop a)

propAnd, propOr           :: Prop alpha -> Prop alpha -> Prop alpha
propAnds, propOrs         :: [Prop alpha] -> Prop alpha
propMap                   :: (alpha -> Prop beta) -> Prop alpha -> Prop beta
propTrue, propFalse       :: Prop alpha
propBool                  :: Bool -> Prop alpha
propLit                   :: alpha -> Prop alpha

-- variable substitution, replacing free variables
class SubstVar a where (/) :: a -> ([VarName],[Expr]) -> a
instance SubstVar Expr
instance SubstVar Alt
instance SubstVar a => SubstVar [a]
instance SubstVar a => SubstVar (Sat a)
instance SubstVar a => SubstVar (Prop a)

-- equality substitution, replacing items
class SubstRep a b c | a c -> b, c b -> a, a b -> c where (/#) :: a -> b -> c
instance SubstRep (Prop (Sat a)) ([a], [b]) (Prop (Sat b))
instance SubstRep VarName ([VarName], [Expr]) Expr

instance Eq Value
instance Eq Expr

alt :: Alt -> Prop (Sat a)
pre' :: String -> [Expr] -> Prop (Sat Expr)
sub :: ([VarName],[Expr])

-- for BP
anys :: String -> Constraint
\end{code}

\h{#mp}\begin{code}
-- for MP
type Constraint = [Val]
data Val = [Pattern] :* [Pattern] | Any
data Pattern = Pattern CtorName [Val]
complete :: CtorName -> Pattern
nonRecs :: CtorName -> [Int]
merge :: [Pattern] -> [Pattern] -> [Pattern]
non :: [Int]
rec :: [Int]
\end{code}
\end{comment}


\chapter{Proof of Pattern-Match Analysis}
\label{chp:proof}

\newcommand{\lemma}[1]{(\textit{#1})}
\newcommand{\theorem}[2]{\lemma{#1} \vspace{-1mm} \\ \nopagebreak #2 }
\newcommand{\proof}[2][]{\textbf{Proof of \lemma{#2} \textsf{#1}} \\  \nopagebreak}

This chapter shows that the algorithms and constraint languages presented in Chapter \ref{chp:catch} are sound -- if Catch informs the user that a program is safe, then that program is guaranteed not to call |error|. The proof is structured as an evaluator for expressions in our Core language, along with a series of theorems about the relationship between the evaluator, the algorithms and the constraint languages.

\section{Notation}

The proof is based on equational reasoning, making use of induction, application of theorems, case analysis and inlining of function definitions. The proof has not been automatically checked. While performing the reasoning steps, we ignore issues such as strictness. All the properties are boolean valued expressions, typically implications.

In order to reduce the size of some of the intermediate expressions, we have replaced one side of an implication with either |lhs| or |rhs|, designating either the left-hand side or right-hand side. We also make heavy use of the function composition and function application operators, namely |(.)| and |($)|. These can be read with the translations:

\ignore\begin{code}
(f . g) x  = f $ g x = f (g x)
\end{code}


\section{Evaluator}

We start with an evaluator for a Core expression language.

\h{#*}\begin{code}
data Value  =  Value CtorName [Value]
            |  Bottom

data Expr  =  Make CtorName [Expr]
           |  Call FuncName [Expr]
           |  Var  VarName
           |  Sel  Expr Selector
           |  Case Expr [Alt]

data Alt = Alt CtorName [VarName] Expr

eval :: Expr -> Value
eval (Sel x (c,i)  )  |  c == c' = xs !! i
    where Value c' xs = eval x
eval (Make c  xs   )  =  Value c (map eval xs)
eval (Call f  xs   )  |  f == "error"  = Bottom
                      |  otherwise     = eval $ body f / (args f, xs)
eval (Case x as    )  =  case eval x of
    Value c xs -> head [eval y | Alt c' vs y <- as, c == c']
    Bottom -> Bottom
\end{code}

The |Expr| data type is based on a first-order variant of the Core language from \S\ref{secB:core}. We have introduced |Sel|, which represents variables bound in case alternatives. For the algorithms presented previously, the |Sel| expression contains the information returned by the |var| function. While evaluating a |Sel| expression we know that we are beneath a |Case| on the same expression |x|, and that |x| evaluates to the constructor mentioned in the selector.

There is no case in |eval| for |Var|, and the behaviour of |eval| with free variables is undefined. The |Call| equation will replace any free variables in the body of a function with the supplied arguments.

We make use of |(/)|, which we have redefined as a substitution operator -- we write |x / (vs,ys)| to denote replacing the free variables |vs| in |x| with |ys|. We use |(/)| instead of |substP| in the proofs, where |substP (zip vs ys) x == x / (vs,ys)|.

We also make use of a number of auxiliaries throughout the proof:

\h{#*}\begin{code}
isBottom :: Value -> Bool
isBottom Bottom = True
isBottom (Value c xs) = any isBottom xs

valCtor :: Value -> Maybe CtorName
valCtor (Value c xs) = Just c
valCtor Bottom = Nothing

propIsTrue :: Prop () -> Bool
propIsTrue = (==) propTrue

propTaut :: (alpha -> Bool) -> Prop alpha -> Bool
propTaut f = propIsTrue . propMap (propBool . f)

satE' :: Prop (Sat Expr) -> Bool
satE' = propTaut satE

satE :: Sat Expr -> Bool
satE (Sat x k) = sat (Sat (eval x) k)

sat' :: Prop (Sat Value) -> Bool
sat' = propTaut sat

sat :: Sat Value -> Bool
sat (Sat Bottom        k) = True
sat (Sat (Value c xs)  k) = sat' $ (c <| k) /# ([0..],xs)
\end{code}

The |sat| function tests whether a value satisfies a constraint, using the |(<||)| operator from the constraint language. The |satE| function tests whether the result of evaluating an expression satisfies a constraint. The |sat'| and |satE'| functions operate over a proposition.

\section{Theorems}

In this section we define several theorems, which we prove in the following sections.

\subsection{Correctness}

The goal of this chapter is to prove correctness, which can be defined as a proof of the following theorem:

\theorem{pre/eval}
{|satE' $ pre x ==> not $ isBottom $ eval x|}

This corresponds to a proof of Figures \ref{figC:property_fixp}, \ref{figC:precondition}, \ref{figC:precond_fixp} and \ref{figC:prop}. This theorem is proved in \S\ref{secP:proof}. To prove safety for a whole program, we can consider the expression |x| to be |Call "main" []|, which is safe if |precond "main" == propTrue|.

\subsection{Constraint Theorems}

We assume the following two theorems about each constraint language:

\theorem{sat/|-<|}
{|sat' (Value c xs -< cs) ==> c `elem` cs|}

\theorem{sat/| ||> |}
{|sat $ Sat (Value c xs) ((c,i) ||> k) ==> sat $ Sat (xs !! i) k|}

Both of these theorems are given in \S\ref{secC:constraint_semantics}, as properties. Note that the definition of |sat| makes use of |(<||)|, so these theorems require the additional two operators to be consistent with |(<||)|. We prove these theorems for the BP-constraint and MP-constraint systems in \S\ref{secP:bp} and \S\ref{secP:mp}. Since RE-constraints do not scale sufficiently, we do not recommend their use, and have therefore not proven them to be consistent.

\subsection{Additional Theorems}

We will also need the following theorems, which we prove in \S\ref{secP:proof}.

\theorem{precond/error}
{|precond "error" == propFalse|}

\theorem{precond}
{|precond f ==> reduce $ pre $ body f|}

\theorem{reduce}
{|satE' $ reduce x /# sub ==> satE' $ x / sub|}

\theorem{red}
{|satE' $ red x k /# sub ==> sat $ Sat (eval $ x / sub) k|}

\theorem{pre}
{|satE' (pre x / (vs, ys)) && all (satE' . pre) ys ==> satE' $ pre $ x / (vs, ys)|}

\theorem{satE/|-<|}
{|sat' (eval x -< cs) == satE' (x -< cs)|}

\theorem{elem}
{|(x `elem` (xs \\ [x])) == False|}

\section{Proofs of Theorems}
\label{secP:proof}

We prove each theorem in turn.

\proof{pre/eval}

\h{expr}\begin{code}
satE' $ pre x ==> not $ isBottom $ eval x
\end{code}

By induction. We do not need to consider |Var| as |eval| cannot be called on expressions with free variables.

\proof[|Sel|]{pre/eval}

The |Sel| equation of |eval| is:

\begin{code}
eval (Sel x (c,i)) | c == c' = xs !! i
    where Value c' xs = eval x
\end{code}

We know that any \ignore|Sel x _| value must be contained within an alternative of a \ignore|Case x _| expression. If we assume that the original |Case| expression satisfied its, we obtain:

\h{exprlist}\begin{code}
satE' $ pre $ Case x as ==> satE' $ pre x
    -- inline |pre|
satE' $ pre x `propAnd` propAnds (map alt as) ==> satE' $ pre x
    -- inline |satE'|
satE' (pre x) && satE' (propAnds $ map alt as) ==> satE' $ pre x
    -- weaken implication
satE' $ pre x ==> satE' $ pre x
    -- equal
True
\end{code}

\proof[|Make|]{pre/eval}

The initial equation is:

\begin{code}
eval (Make c xs) = Value c (map eval xs)
\end{code}

This does not produce |Bottom| if all recursive calls to |eval| are on values which satisfy |pre|. We can write this as:

\h{exprlist}\begin{code}
satE' $ pre $ Make c xs  ==> all (satE' . pre) xs
    -- inline |pre|
satE' $ propAnds $ map pre xs ==> all (satE' . pre) xs
    -- inline |satE'|
and $ map satE' $ map pre xs  ==> all (satE' . pre) xs
    -- |map f . map g == map (f . g)|
and $ map (satE' . pre) xs ==> all (satE' . pre) xs
    -- |and . map f == all f|
all (satE' . pre) xs ==> all (satE' . pre) xs
    -- equal
True
\end{code}

\proof[|Call|]{pre/eval}

The initial equation is:

\begin{code}
eval (Call f xs)  | f == "error" = Bottom
                  | otherwise = eval $ body f / (args f, xs)
\end{code}

There are two ways to that |Bottom| may occur in this fragment. The first is the explicit |Bottom|, and the second is the recursive call to |eval|. The explicit |Bottom| is avoided under the condition:

\h{exprlist}\begin{code}
satE' $ pre $ Call f xs ==> f /= "error"
    -- inline |pre|
satE' $ (precond f /# (args f, xs)) `propAnd` propAnds (map pre xs) ==> f /= "error"
    -- inline |satE'|
satE' (precond f /# (args f, xs)) && all (satE' . pre) xs ==> f /= "error"
    -- weaken implication
satE' (precond f /# (args f, xs)) ==> f /= "error"
\end{code}

We can now perform case analysis on |f|, assuming it either is, or is not, equal to |"error"|.

\h{exprlist}\begin{code}
satE' (precond f /# (args f, xs)) ==> f /= "error"
    -- assume |f /= "error"|
satE' (precond f /# (args f, xs)) ==> True
    -- implication
True
\end{code}

\h{exprlist}\begin{code}
satE' (precond f /# (args f, xs)) ==> f /= "error"
    -- assume |f == "error"|
satE' (precond f /# (args f, xs)) ==> False
    -- implication
not $ satE' (precond "error" /# (args f, xs))
    -- \lemma{precond/error}
not $ satE' $ (propFalse /# (args f, xs))
    -- inline |(/)|
not $ satE' propFalse
    -- inline |satE'|
not $ False
    -- inline |not|
True
\end{code}

This leaves us with the call to |eval|, namely:

\h{exprlist}\begin{code}
satE' $ pre $ Call f xs ==> satE' $ pre $ body f / (args f, xs)
    -- inline pre on LHS
satE' $ (precond f /# (args f, xs)) `propAnd` propAnds (map pre xs) ==> rhs
    -- inline |satE'|
satE' (precond f /# (args f, xs)) && all (satE' . pre) xs ==> rhs
    -- \lemma{precond}
satE' ((reduce $ pre $ body f) /# (args f, xs)) && all (satE' . pre) xs ==> rhs
    -- \lemma{reduce}
satE' (pre (body f) / (args f, xs)) && all (satE' . pre) xs ==> rhs
    -- \lemma{pre/subst}
satE' $ pre $ body f / (args f, xs) ==> satE' $ pre $ body f / (args f, xs)
    -- equal
True
\end{code}

\proof[|Case|]{pre/eval}

The |Case| equation is:

\begin{code}
eval (Case x as) = case eval x of
    Value c xs -> head [eval y | Alt c' vs y <- as, c == c']
    Bottom -> Bottom
\end{code}

This equation may generate |Bottom| in two ways -- either the explicit |Bottom| may be taken, or the recursive call to |eval| may result in |Bottom|. In both cases, if we can prove the expression passed to |eval| satisfies its precondition, then we can eliminate the possibility of |Bottom|.

We first prove that the explicit |Bottom| is not reached, assuming the initial expression does not violate the precondition check.

\h{exprlist}\begin{code}
satE' $ pre $ Case x as ==> satE' $ pre x
    -- inline |pre|
satE' $ pre x `propAnd` propAnds (map alt as) ==> satE' $ pre x
    -- inline |satE'|
satE' (pre x) && satE' (propAnds $ map alt as) ==> satE' $ pre x
    -- weaken implication
satE' $ pre x ==> satE' $ pre x
    -- equal
True
\end{code}

We now need to ensure that the other call to |eval| meets its precondition.

\h{exprlist}\begin{code}
satE' $ pre $ Case x as ==>
    all (\(Alt c vs y) -> valCtor (eval x) == Just c ==> satE' $ pre y) as
    -- inline |pre|
satE' $ pre x `propAnd` propAnds (map alt as) ==> rhs
    -- inline |satE'|
satE' (pre x) && all (satE' . alt) as ==> rhs
    -- weaken implication
all (satE' . alt) as ==>
    all (\(Alt c vs y) -> valCtor (eval x) == Just c ==> satE' $ pre y) as
    -- lift implies over all
satE' $ alt a ==> (\(Alt c vs y) -> valCtor (eval x) == Just c ==> satE' $ pre y) a
    -- instantiate |a == Alt c v ys|
satE' $ alt $ Alt c v ys ==> (valCtor (eval x) == Just c ==> satE' $ pre y)
    -- inline |alt|
satE' (x -< (ctors c \\ [c]) `propOr` pre y) ==> rhs
    -- inline |satE'|
satE' (x -< (ctors c \\ [c])) || satE' (pre y) ==> rhs
    -- \lemma{satE/|-<|}
sat' (eval x -< (ctors c \\ [c])) || satE' (pre y) ==> rhs
    -- using |valCtor (eval x) == Just c|
    -- we infer |eval x == Value c ys|
sat' (Value c ys -< (ctors c \\ [c])) || satE' (pre y) ==> satE' $ pre y
    -- \lemma{sat/|-<|}
c `elem` (ctors c \\ [c]) || satE' (pre y) ==> satE' $ pre y
    -- \lemma{elem}
False || satE' (pre y) ==> satE' $ pre y
    -- inline |(||||)|
satE' $ pre y ==> satE' $ pre y
    -- equals
True
\end{code}


\proof{elem}

\h{expr}\begin{code}
(x `elem` (ys \\ [x])) == False
\end{code}

The |elem| application is only true if |ys \\ [x]| contains |x|. The expression cannot contain |x|, as if it existed in |ys| it was removed, therefore this application is always |False|.

\proof{precond/error}

\h{expr}\begin{code}
precond "error" == propFalse
\end{code}

The initial computation of |precond| will return |propFalse|. All successive computations will be at least as restrictive, therefore the result must be |propFalse|.

\proof{precond}

\h{expr}\begin{code}
precond f ==> reduce $ pre $ body f
\end{code}

The definition of |precond f| is a conjunction where the second conjunct is |reduce $ pre $ body f|, therefore |precond f| is at least as restrictive as the alternative.


\proof{satE/|-<|}

\h{exprlist}\begin{code}
sat' (eval x -< cs) == satE' (x -< cs)
    -- inline |sat'| and |satE'|
propTaut sat (eval x -< cs) == propTaut satE (x -< cs)
    -- inline |propTaut| and reduce common bits
propMap (propBool . sat) (eval x -< cs) == propMap (propBool . satE) (x -< cs)
\end{code}

Now we can use the type signature of |-<|:

\begin{code}
(-<) :: alpha -> [CtorName] -> Prop (Sat alpha)
\end{code}

The theorems for free work \cite{wadler:theorems} shows that the first argument will end up as the first argument of the |Sat| constructor, unmodified and unexamined. The |satE| function applies |eval| to the first argument of |Sat|, therefore both these pieces of code are equivalent.


\proof{pre}

\h{exprlist}\begin{code}
satE' (pre x / (vs, ys)) && all (satE' . pre) ys ==> satE' $ pre $ x / (vs, ys)
\end{code}

This proof is by case analysis on |x|. We assume that all free variables in |x| are bound in |vs|. To shorten the proofs we do not explicitly write the |all (satE' . pre) ys| term, as it is never manipulated.

\proof[|Var|]{pre}

\h{exprlist}\begin{code}
satE' $ pre x / (vs, ys) ==> satE' $ pre $ x / (vs, ys)
    -- |x == Var v|
satE' $ pre (Var v) / (vs, ys) ==> satE' $ pre $ Var v / (vs, ys)
    -- inline |pre| on LHS
satE' $ propTrue / (vs, ys) ==> satE' $ pre $ Var v / (vs, ys)
    -- inline |(/)| on LHS
satE' propTrue ==> satE' $ pre $ Var v / (vs, ys)
    -- inline |satE'|
True ==> satE' $ pre $ Var v / (vs, ys)
    -- reintroduce hidden term
all (satE' . pre) ys ==> satE' $ pre $ Var v / (vs, ys)
\end{code}

We know that |v| will be a member of |vs|, and that the result will be |pre y|, where |y| is drawn from |ys|. Since all |ys| satisfy the precondition, then so will the particular |y| we substitute.

\proof[|Sel|]{pre}

\h{exprlist}\begin{code}
satE' $ pre x / (vs, ys) ==> satE' $ pre $ x / (vs, ys)
    -- |x == Sel x s|
satE' $ pre (Sel x s) / (vs, ys) ==> satE' $ pre $ Sel x s / (vs, ys)
    -- inline |(/)| on RHS
satE' $ pre (Sel x s) / (vs, ys) ==> satE' $ pre $ Sel (x / (vs,ys)) s
    -- inline |pre| on RHS
satE' $ pre (Sel x s) / (vs, ys) ==> satE' $ propTrue
    -- inline |satE'| on RHS
satE' $ pre (Sel x s) / (vs, ys) ==> True
    -- implication
True
\end{code}

\proof[|Make|]{pre}

\h{exprlist}\begin{code}
satE' $ pre x / (vs, ys) ==> satE' $ pre $ x / (vs, ys)
    -- |x == Make c xs|
satE' $ pre (Make c xs) / (vs, ys) ==> satE' $ pre $ Make c xs / (vs, ys)
    -- inline |(/)| on RHS
satE' $ pre (Make c xs) / (vs, ys) ==>
    satE' $ pre $ Make c $ map (/ (vs, ys)) xs
    -- inline |pre| on both sides
satE' $ propAnds (map pre xs) / (vs, ys) ==>
    satE' $ propAnds $ map (pre . (/ (vs, ys))) xs
    -- inline |(/)| on LHS
satE' $ propAnds $ map ((/ (vs,ys)) . pre) xs ==>
    satE' $ propAnds $ map (pre . (/ (vs, ys))) xs
    -- inline |satE'| on both sides
all (satE' . (/ (vs,ys)) . pre) xs ==> all (satE' . pre . (/ (vs, ys))) xs
    -- \lemma{pre}
True
\end{code}

\proof[|Call|]{pre}

\h{exprlist}\begin{code}
satE' $ pre x / (vs, ys) ==> satE' $ pre $ x / (vs, ys)
    -- |x == Call f xs|
satE' $ pre (Call f xs) / (vs, ys) ==> satE' $ pre $ Call f xs / (vs, ys)
    -- inline |(/)| on RHS
satE' $ pre (Call f xs) / (vs, ys) ==> satE' $ pre $ Call f $ map (/ (vs, ys)) xs
\end{code}

Now we will work on each side individually, starting with LHS:

\h{exprlist}\begin{code}
satE' $ pre (Call f xs) / (vs, ys)
    -- inline |pre|
satE' $ (pre' f xs `propAnd` propAnds (map pre xs)) / (vs,ys)
    -- inline |(/)|
satE' $ (pre' f xs / (vs,ys)) `propAnd` propAnds (map (pre . (/ (vs,ys))) xs)
    -- inline |satE'|
satE' (pre' f xs / (vs,ys)) && all (satE' . pre . (/ (vs,ys))) xs
\end{code}

And the RHS:

\h{exprlist}\begin{code}
satE' $ pre $ Call f $ map (/ (vs, ys)) xs
    -- inline |pre|
satE' $ (pre' f (map (/ (vs, ys)) xs)) `propAnd` propAnds (map (pre . (/ (vs, ys))) xs)
    -- inline |satE'|
satE' (pre' f (map (/ (vs, ys)) xs)) && all (satE' . pre . (/ (vs, ys))) xs
\end{code}

We can now combine these sides, eliminating the common term:

\h{exprlist}\begin{code}
satE' $ pre' f xs / (vs,ys) ==> satE' $ pre' f (map (/ (vs, ys)) xs)
    -- inline |pre'|
satE' $ (precond f /# (args f, xs)) / (vs,ys) ==>
    satE' $ precond f /# (args f, map (/ (vs, ys)) xs)
    -- using the knowledge that |precond f| only has free variables in |args f|
    -- we can inline |(/)| on the LHS
satE' $ precond f /# (args f, map (/ (vs,ys)) xs) ==>
    satE' $ precond f /# (args f, map (/ (vs, ys)) xs)
    -- equal
True
\end{code}

\proof[|Case|]{pre}

\h{exprlist}\begin{code}
satE' $ pre x / (vs, ys) ==> satE' $ pre $ x / (vs, ys)
    -- |x == Case x as|
satE' $ pre (Case x as) / (vs, ys) ==> satE' $ pre $ Case x as / (vs, ys)
    -- inline |(/)| on RHS
satE' $ pre (Case x as) / (vs, ys) ==>
    satE' $ pre $ Case (x / (vs, ys)) (map (/ (vs, ys)) as)
    -- inline |pre| on both sides
satE' $ (pre x `propAnd` propAnds (map alt as)) / (vs, ys) ==>
    satE' $ pre (x / (vs, ys)) `propAnd` propAnds (map (alt . (/ (vs, ys))) as)
    -- inline |(/)| on LHS
satE' $ (pre x / (vs, ys)) `propAnd` propAnds (map ((/ (vs, ys)) . alt) as)  ==>
    satE' $ pre (x / (vs, ys)) `propAnd` propAnds (map (alt . (/ (vs, ys))) as)
    -- inline |satE'|
satE' (pre x / (vs, ys)) && all (satE' . (/ (vs, ys)) . alt) as ==>
    satE' (pre (x / (vs, ys))) && all (satE' . alt . (/ (vs, ys))) as
    -- \lemma{pre}
all (satE' . (/ (vs, ys)) . alt) as  ==> all (satE' . alt . (/ (vs, ys))) as
    -- implication over |all|
satE' $ alt a / (vs, ys) ==> satE' $ alt $ as / (vs, ys)
    -- instantiate |a| as a general |Alt|
satE' $ alt (Alt c ws y) / (vs, ys) ==> satE' $ alt $ Alt c ws y / (vs, ys)
    -- inline |(/)| on RHS
satE' $ alt (Alt c ws y) / (vs, ys) ==> satE' $ alt $ Alt c ws (y / (vs, ys))
    -- inline |alt|
satE' $ (x -< (ctors c \\ [c]) `propOr` pre y) / (vs, ys) ==>
    satE' $ (x / (vs,ys) -< (ctors c \\ [c])) `propOr` pre (y / (vs, ys))
    -- let |cs == ctors c \\ [c]|
satE' $ (x -< cs `propOr` pre y) / (vs, ys) ==>
    satE' $ (x / (vs,ys) -< cs) `propOr` pre (y / (vs, ys))
    -- inline |(/)| on LHS
satE' $ (x / (vs,ys) -< cs) `propOr` (pre y / (vs, ys)) ==>
    satE' $ (x / (vs,ys) -< cs) `propOr` pre (y / (vs, ys))
    -- inline |satE'| on both sides
satE' (x / (vs,ys) -< cs) || satE' (pre y / (vs, ys)) ==>
    satE' (x / (vs,ys) -< cs) || satE' (pre (y / (vs, ys)))
    -- remove duplicate bits on each side
satE' $ pre y / (vs, ys) ==> satE' $ pre $ y / (vs, ys)
    -- \lemma{pre}
True
\end{code}


\proof{reduce}

\h{exprlist}\begin{code}
satE' $ reduce x /# sub ==> satE' $ x / sub
    -- inline |reduce|
satE' $ propMap (\(Sat x k) -> red x k) x /# sub ==> satE' $ x / sub
    -- inline |(/)| on LHS
satE' $ propMap (\(Sat x k) -> red x k /# sub) x ==> satE' $ x / sub
    -- inline |(/)| on RHS
satE' $ propMap (\(Sat x k) -> red x k /# sub) x ==>
    satE' $ propMap (\(Sat x k) -> propLit $ Sat x k / sub) x
    -- inline |(/)| on RHS
satE' $ propMap (\(Sat x k) -> red x k /# sub) x ==>
    satE' $ propMap (\(Sat x k) -> propLit $ Sat (x / sub) k) x
    -- inline |satE'|
propIsTrue $ propMap (\(Sat x k) -> propBool $ satE' $ red x k /# sub) x ==>
    propIsTrue $ propMap (\(Sat x k) -> propBool $ satE' $ propLit $ Sat (x / sub) k) x
    -- lift |propMap| over |(==>)|
satE' $ red x k /# sub ==> satE' $ propLit $ Sat (x / sub) k
    -- inline |satE'| on RHS
satE' $ red x k /# sub ==> satE $ Sat (x / sub) k
    -- inline |satE| on RHS
satE' $ red x k /# sub ==> sat $ Sat (eval $ x / sub) k
    -- \lemma{red}
True
\end{code}


\proof{red}

\h{expr}\begin{code}
satE' $ red x k /# sub ==> sat $ Sat (eval $ x / sub) k
\end{code}

We prove by case analysis on the expression |x|.

\proof[|Var|]{red}

\h{exprlist}\begin{code}
satE' $ red x k /# sub ==> sat $ Sat (eval $ x / sub) k
    -- |x == Var v|
satE' $ red (Var v) k /# sub ==> sat $ Sat (eval $ Var v / sub) k
    -- inline |red|
satE' $ propLit (Sat v k) /# sub ==> sat $ Sat (eval $ Var v / sub) k
    -- inline |(/)| on LHS
satE' $ propLit (Sat (v /# sub) k) ==> sat $ Sat (eval $ Var v / sub) k
    -- promote |v| on LHS to |Var v|
    -- because |(/)| operates identically on both
satE' $ propLit (Sat (Var v / sub) k) ==> sat $ Sat (eval $ Var v / sub) k
    -- inline |satE'|
satE (Sat (Var v / sub) k) ==> sat $ Sat (eval $ Var v / sub) k
    -- inline |satE|
sat $ Sat (eval $ Var v / sub) k ==> sat $ Sat (eval $ Var v / sub) k
    -- equal
True
\end{code}

\proof[|Sel|]{red}

In this proof, we assume |eval (x / sub) == Value c xs|, due to being in the alternative of a |Case| expression.

\h{exprlist}\begin{code}
satE' $ red x k /# sub ==> sat $ Sat (eval $ x / sub) k
    -- |x == Sel x (c,i)|
satE' $ red (Sel x (c,i)) k /# sub ==> sat $ Sat (eval $ Sel x (c,i) / sub) k
    -- inline |red|
satE' $ red x ((c,i) |> k) /# sub ==> sat $ Sat (eval $ Sel x (c,i) / sub) k
    -- inline |(/)| on RHS
satE' $ red x ((c,i) |> k) /# sub ==> sat $ Sat (eval $ Sel (x / sub) (c,i)) k
    -- inline |eval| on RHS
satE' $ red x ((c,i) |> k) /# sub ==> sat $ Sat (xs !! i) k
    -- \lemma{sat/| ||> |}
satE' $ red x ((c,i) |> k) /# sub ==> sat $ Sat (Value c xs) ((c,i) |> k)
    -- replace using the assumption
satE' $ red x ((c,i) |> k) /# sub ==> sat $ Sat (eval (x / sub)) ((c,i) |> k)
    -- \lemma{red}
True
\end{code}

\proof[|Make|]{red}

\h{exprlist}\begin{code}
satE' $ red x k /# sub ==> sat $ Sat (eval $ x / sub) k
    -- |x == Make c xs|
satE' $ red (Make c xs) k /# sub ==> sat $ Sat (eval $ Make c xs / sub) k
    -- inline |red|
satE' $ reduce ((c <| k) /# ([0..], xs)) /# sub ==> sat $ Sat (eval $ Make c xs / sub) k
    -- \lemma{reduce}
satE' $ ((c <| k) /# ([0..], xs)) / sub ==> sat $ Sat (eval $ Make c xs / sub) k
    -- inline |(/)| on LHS
satE' $ (c <| k) /# ([0..], map (/ sub) xs) ==> sat $ Sat (eval $ Make c xs / sub) k
    -- inline |satE'| on LHS
sat' $ (c <| k) /# ([0..], map (eval . (/ sub)) xs) ==>
    sat $ Sat (eval $ Make c xs / sub) k
    -- inline |(/)| on RHS
sat' $ (c <| k) /# ([0..], map (eval . (/ sub)) xs) ==>
    sat $ Sat (eval $ Make c (map (/ sub) xs)) k
    -- inline |eval| on RHS
sat' $ (c <| k) /# ([0..], map (eval . (/ sub)) xs) ==>
    sat $ Sat (Value c (map (eval . (/ sub)) xs)) k
    -- fold back |sat|
sat $ Sat (Value c (map (eval . (/ sub)) xs)) k ==>
    sat $ Sat (Value c (map (eval . (/ sub)) xs)) k
    -- equal
True
\end{code}

\proof[|Call|]{red}

\h{exprlist}\begin{code}
satE' $ red x k /# sub ==> sat $ Sat (eval $ x / sub) k
    -- |x == Call f xs|
satE' $ red (Call f xs) k /# sub ==> sat $ Sat (eval $ Call f xs / sub) k
    -- inline |red|
satE' $ reduce (prePost f k /# (args f, xs)) /# sub ==> rhs
    -- \lemma{reduce}
satE' $ (prePost f k /# (args f, xs)) / sub ==> rhs
    -- inline |(/)| on LHS
satE' $ prePost f k /# (args f, map (/sub) xs) ==> rhs
    -- \lemma{prePost}
satE' $ reduce (propLit $ Sat (body f) k) /# (args f, map (/sub) xs) ==> rhs
    -- \lemma{reduce}
satE' $ (propLit $ Sat (body f) k) / (args f, map (/sub) xs) ==> rhs
    -- inline |(/)| on LHS
satE' $ (propLit $ Sat (body f / (args f, map (/sub) xs)) k) ==> rhs
    -- inline |satE'|
satE $ Sat (body f / (args f, map (/sub) xs)) k ==> rhs
    -- inline |satE|
sat $ Sat (eval $ body f / (args f, map (/sub) xs)) k ==>
    sat $ Sat (eval $ Call f xs / sub) k
    -- inline |(/)| on RHS
sat $ Sat (eval $ body f / (args f, map (/sub) xs)) k ==>
    sat $ Sat (eval $ Call f (map (/ sub) xs)) k
\end{code}

We now assume that either |f| is equal to error, or not.

\h{exprlist}\begin{code}
sat $ Sat (eval $ body f / (args f, map (/ sub) xs)) k ==>
    sat $ Sat (eval $ Call f (map (/ sub) xs)) k
    -- assume |f == "error"|
sat $ Sat (eval $ body "error" / (args f, map (/ sub) xs)) k ==>
    sat $ Sat (eval $ Call "error" (map (/ sub) xs)) k
    -- inline |eval| on RHS
sat $ Sat (eval $ body "error" / (args f, map (/ sub) xs)) k ==>
    sat $ Sat Bottom k
    -- inline |sat|
sat $ Sat (eval $ Call "error" [Var "x"] / (["x"], map (/sub) xs)) k ==> False
    -- implies
True
\end{code}

\h{exprlist}\begin{code}
sat $ Sat (eval $ body f / (args f, map (/ sub) xs)) k ==>
    sat $ Sat (eval $ Call f (map (/ sub) xs)) k
    -- inline |eval| on RHS, assuming |f /= "error"|
sat $ Sat (eval $ body f / (args f, map (/ sub) xs)) k ==>
    sat $ Sat (eval $ body f / (args f, map (/ sub) xs)) k
    -- equal
True
\end{code}

\proof[|Case|]{red}

\h{exprlist}\begin{code}
satE' $ red x k /# sub ==> sat $ Sat (eval $ x / sub) k
    -- |x == Case x as|
satE' $ red (Case x as) k /# sub ==> sat $ Sat (eval $ Case x as / sub) k
    -- inline |red|
satE' $ propAnds (map alt as) /# sub ==> sat $ Sat (eval $ Case x as / sub) k
    -- inline |(/)| on LHS
satE' $ propAnds $ map ((/# sub) . alt) as ==> sat $ Sat (eval $ Case x as / sub) k
    -- inline |satE'|
all (satE' . (/# sub) . alt) as ==> sat $ Sat (eval $ Case x as / sub) k
    -- inline |(/)| on RHS
all (satE' . (/# sub) . alt) as ==> sat $ Sat (eval $ Case (x / sub) (as / sub)) k
\end{code}

First assume that |eval (x / sub) == Bottom|, then that |eval (x / sub) == Value c xs|.

\h{exprlist}\begin{code}
all (satE' . (/# sub) . alt) as ==> sat $ Sat (eval $ Case (x / sub) (as / sub)) k
    -- inline |eval|, assuming |eval (x / sub) == Bottom|
all (satE' . (/# sub) . alt) as ==> sat $ Sat Bottom k
    -- inline |sat|
all (satE' . (/# sub) . alt) as ==> True
    -- implies
True
\end{code}

\h{exprlist}\begin{code}
all (satE' . (/# sub) . alt) as ==> sat $ Sat (eval $ Case (x / sub) (as / sub)) k
    -- inline |eval|, assuming |eval (x / sub) == Value c xs|
lhs ==> sat $ Sat (head [eval y | Alt c' vs y <- as / sub, c == c']) k
    -- expand RHS, removing list comprehension
all (satE' . (/# sub) . alt) as ==>
    all (\(Alt c' vs y) -> c == c' ==> sat $ Sat (eval y) k) (as / sub)
    -- lift implication over |all|
satE' $ alt a /# sub ==>
    (\(Alt c' vs y) -> c == c' ==> sat $ Sat (eval y) k) (a / sub)
    -- instantiate |a == Alt c' vs y|
satE' $ alt a /# sub ==>
    (\(Alt c' vs y) -> c == c' ==> sat $ Sat (eval y) k) (Alt c' vs y / sub)
    -- inline |(/)| on RHS
satE' $ alt a /# sub ==>
    (\(Alt c' vs y) -> c == c' ==> sat $ Sat (eval y) k) (Alt c' vs $ y / sub)
    -- inline lambda on RHS
satE' $ alt (Alt c' vs y) /# sub ==>
    (c == c' ==> sat $ Sat (eval $ y / sub) k)
    -- use knowledge from RHS in LHS
satE' $ alt (Alt c vs y) /# sub ==> sat $ Sat (eval $ y / sub) k
    -- inline |alt| on LHS
satE' $ (reduce (x -< (ctors c \\ [c])) `propOr` red y k) /# sub ==> rhs
    -- inline |(/)| on LHS
satE' $ (reduce (x -< (ctors c \\ [c])) /# sub) `propOr` (red y k /# sub) ==> rhs
    -- inline |satE'| on LHS
satE' (reduce (x -< (ctors c \\ [c])) /# sub) || satE' (red y k /# sub) ==> rhs
    -- \lemma{reduce}
satE' ((x -< (ctors c \\ [c])) / sub) || satE' (red y k /# sub) ==> rhs
    -- inline |(/)| on LHS
satE' ((x / sub) -< (ctors c \\ [c])) || satE' (red y k /# sub) ==> rhs
    -- \lemma{satE/|-<|}
sat' (eval (x / sub) -< (ctors c \\ [c])) || satE' (red y k /# sub) ==> rhs
    -- substitute |eval (x / sub) == Value c xs|
sat' (Value c xs -< (ctors c \\ [c])) || satE' (red y k /# sub) ==> rhs
    -- \lemma{sat/|-<|}
c `elem` (ctors c \\ [c]) || satE' (red y k /# sub) ==> rhs
    -- \lemma{elem}
False || satE' (red y k /# sub) ==> rhs
    -- inline |(||||)|
satE' $ red y k /# sub ==> sat $ Sat (eval $ y / sub) k
    -- \lemma{red}
True
\end{code}

\section{Correctness of BP-constraints}
\label{secP:bp}

Since BP-constraints are presented piecemeal throughout \S\ref{secC:manipulate}, we recap them here:

\begin{code}
data Constraint  =  Any
                 |  Con CtorName [Constraint]

a -< xs = propOrs [propLit (a `Sat` anys x) | x <- xs]
    where anys x = Con x (replicate (arity x) Any)

(c,i) |> k = Con c  [  if i == j then k else Any
                    |  j <- [0..arity c - 1]]

c <| Any         =  propTrue
c <| Con c_2 xs  =  propBool (c_2 == c) `propAnd` propAnds (map propLit (zipWith Sat [0..] xs))
\end{code}

\proof{sat/|-<|}

\h{exprlist}\begin{code}
sat' (Value c xs -< cs) ==> c `elem` cs
    -- inline |(-<)|
sat' $ propOrs [propLit (Value c xs `Sat` anys c') | c' <- cs] ==> c `elem` cs
    -- inline |sat'|
any (\c' -> sat $ Value c xs `Sat` anys c') cs ==> c `elem` cs
    -- inline |sat|
any (\c' -> sat' $ (c <| anys c') /# ([0..],xs)) cs ==> c `elem` cs
    -- inline |anys|
any (\c' -> sat' $ (c <| Con c' (replicate (arity c') Any)) /#
    ([0..],xs)) cs ==> c `elem` cs
    -- inline | <|| |
any (\c' -> sat' $ (propBool (c' == c) `propAnd`
    propAnds (map propLit (zipWith Sat [0..] (replicate (arity c') Any))))
    /# ([0..],xs)) cs ==> c `elem` cs
    -- inline |(/)|
any (\c' -> sat' $ (propBool (c' == c) `propAnd`
    propAnds (map propLit (zipWith Sat [0..] (replicate (arity c') Any)
    /# ([0..],xs))))) cs ==> c `elem` cs
    -- inline |sat'|
any (\c' -> (c' == c) && all sat (zipWith Sat [0..] (replicate (arity c') Any)
    /# ([0..],xs))) cs ==> c `elem` cs
    -- weaken implication
any (\c' -> c' == c) cs ==> c `elem` cs
    -- simplify
any (== c) cs ==> c `elem` cs
    -- definition of |elem|
c `elem` cs ==> c `elem` cs
    -- equal
True
\end{code}

\proof{sat/| ||> |}

By case analysis on |k|, first |Any| then |Con c' ys|.

\proof[|Any|]{sat/| ||> |}

\h{exprlist}\begin{code}
sat $ Sat (Value c xs) ((c,i) |> k) ==> sat $ Sat (xs !! i) k
    -- |k == Any|
sat $ Sat (Value c xs) ((c,i) |> Any) ==> sat $ Sat (xs !! i) Any
    -- inline |sat| on RHS
sat $ Sat (Value c xs) ((c,i) |> Any) ==> sat $ Sat (xs !! i) Any
\end{code}

Now by analysis on |xs !! i|, being either |Value c' ys| or |Bottom|.

\h{exprlist}\begin{code}
sat $ Sat (Value c xs) ((c,i) |> Any) ==> sat $ Sat (xs !! i) Any
    -- |xs !! i == Bottom|
sat $ Sat (Value c xs) ((c,i) |> Any) ==> sat $ Sat Bottom Any
    -- inline |sat| on RHS
sat $ Sat (Value c xs) ((c,i) |> Any) ==> True
    -- implication
True
\end{code}

\h{exprlist}\begin{code}
sat $ Sat (Value c xs) ((c,i) |> Any) ==> sat $ Sat (xs !! i) Any
    -- |xs !! i == Value c' ys|
sat $ Sat (Value c xs) ((c,i) |> Any) ==> sat $ Sat (Value c' ys) Any
    -- inline |sat| on RHS
sat $ Sat (Value c xs) ((c,i) |> Any) ==> sat' $ (c' <| Any) /# ([0..],ys)
    -- inline | <|| |
sat $ Sat (Value c xs) ((c,i) |> Any) ==> sat' $ propTrue /# ([0..],ys)
    -- inline |(/)| on RHS
sat $ Sat (Value c xs) ((c,i) |> Any) ==> sat' propTrue
    -- inline |sat'| on RHS
sat $ Sat (Value c xs) ((c,i) |> Any) ==> True
    -- implication
True
\end{code}

\proof[|Con|]{sat/| ||> |}

\h{exprlist}\begin{code}
sat $ Sat (Value c xs) ((c,i) |> k) ==> sat $ Sat (xs !! i) k
    -- |k == Con c' ys|
sat $ Sat (Value c xs) ((c,i) |> Con c' ys) ==> sat $ Sat (xs !! i) (Con c' ys)
    -- inline |sat| on LHS
sat' $ (c <| ((c,i) |> Con c' ys)) /# ([0..],xs) ==> rhs
    -- inline | ||> |
sat' $ (c <| (Con c [if i == j then (Con c' ys) else Any | j <- [0..arity c - 1]]))
    /# ([0..],xs) ==> rhs
    -- inline | <|| |
sat' $ (propBool (c == c) `propAnd` propAnds (map propLit (zipWith Sat [0..]
    [if i == j then (Con c' ys) else Any | j <- [0..arity c - 1]])))
    /# ([0..],xs) ==> rhs
    -- inline |c == c|
sat' $ (propTrue `propAnd` propAnds (map propLit (zipWith Sat [0..]
    [if i == j then (Con c' ys) else Any | j <- [0..arity c - 1]])))
    /# ([0..],xs) ==> rhs
    -- inline |propAnd|
sat' $ (propAnds (map propLit (zipWith Sat [0..]
    [if i == j then (Con c' ys) else Any | j <- [0..arity c - 1]])))
    /# ([0..],xs) ==> rhs
    -- inline |(/)|
sat' $ propAnds $ map propLit $ zipWith Sat [0..]
    [if i == j then (Con c' ys) else Any | j <- [0..arity c - 1]] /# ([0..],xs) ==> rhs
    -- inline |sat'|
all sat $ zipWith Sat [0..]
    [if i == j then (Con c' ys) else Any | j <- [0..arity c - 1]] /# ([0..],xs) ==> rhs
    -- inline |(/)|
all sat $ zipWith Sat xs
    [if i == j then (Con c' ys) else Any | j <- [0..arity c - 1]] ==> rhs
    -- weaken LHS
sat $ zipWith Sat xs
    [if i == j then (Con c' ys) else Any | j <- [0..arity c - 1]] !! i ==> rhs
    -- inline |(!!)|
sat $ Sat (xs !! i) (Con c' ys) ==> rhs
    -- restore RHS
sat $ Sat (xs !! i) (Con c' ys) ==> sat $ Sat (xs !! i) (Con c' ys)
    -- equal
True
\end{code}

\section{Correctness of MP-constraints}
\label{secP:mp}

This section corresponds to a proof of the code contained in Figure \ref{figC:enumeration}. To perform some of these proofs, we will rely on the following theorems about MP-constraints:

\theorem{sat/any}
{\h{#mp}|sat (Sat (Value c xs) ks) == any (\k -> sat $ Sat (Value c xs) [k]) ks|}

\lemma{sat/merge1}
\vspace{-5mm}
\h{#mp}\begin{code}
sat $ Sat (Value c xs) [merge ms_1 m :* ms_2] ==>
    sat $ Sat (Value c xs) [ms_1 :* ms_2]
\end{code}

\lemma{sat/merge2}
\vspace{-5mm}
\h{#mp}\begin{code}
sat $ Sat (Value c xs) [ms_1 :* merge m ms_2] ==>
    sat $ Sat (Value c xs) [ms_1 :* ms_2]
\end{code}

\proof{sat/any}

\h{#mp exprlist}\begin{code}
sat (Sat (Value c xs) ks) == any (\k -> sat $ Sat (Value c xs) [k]) ks
    -- inline |sat|
sat' ((c <| ks) /# ([0..],xs)) == rhs
    -- inline | <|| |
sat' (propOrs (map f ks) /# ([0..],xs)) == rhs
    -- inline |(/)|
sat' (propOrs (map f ks /# ([0..],xs))) == rhs
    -- inline |sat'|
any sat' (map f ks /# ([0..],xs)) == rhs
    -- inline |(/)|
any sat' (map ((/# ([0..],xs)) . f) ks) == rhs
    -- combine |any| and |map|
any (sat' . (/# ([0..],xs)) . f) ks == rhs
    -- insert |k|
any (\k -> sat' $ f k /# ([0..],xs)) ks == rhs
    -- insert RHS
any (\k -> sat' $ f k /# ([0..],xs)) ks == any (\k -> sat $ Sat (Value c xs) [k]) ks
    -- unwrap common parts
sat' (f k /# ([0..],xs)) == sat (Sat (Value c xs) [k])
    -- inline |sat|
lhs == sat' ((c <| [k]) /# ([0..],xs))
    -- inline | <|| |
lhs == sat' (propOrs (map f [k]) /# ([0..],xs))
    -- inline |map|
lhs == sat' (propOrs [f k] /# ([0..],xs))
    -- inline |propOrs|
sat' (f k /# ([0..],xs)) == sat' (f k /# ([0..],xs))
    -- equal
True
\end{code}


\proof{sat/merge1}

\h{#mp exprlist}\begin{code}
sat $ Sat (Value c xs) [ms_1 :* ms_2]
    -- inline |sat|
sat' $ (c <| [ms_1 :* ms_2]) /# ([0..],xs)
    -- inline | <|| |
sat' $ propOrs (map f [ms_1 :* ms_2]) /# ([0..],xs)
    -- inline |map|
sat' $ propOrs [f $ merge ms_1 m :* ms_2] /# ([0..],xs)
    -- inline |propOrs|
sat' $ (f $ merge ms_1 m :* ms_2) /# ([0..],xs)
    -- inline |f|
sat' $ propOrs [propAnds $ map propLit $ g vs_1 | Pattern c_1 vs_1 <- merge ms_1 m, c_1 == c] /# ([0..],xs)
    -- inline |(/)|
sat' $ propOrs [propAnds $ map propLit $ g vs_1  /# ([0..],xs) | Pattern c_1 vs_1 <- merge ms_1 m, c_1 == c]
    -- inline |sat'|
or [all sat' $ g vs_1  /# ([0..],xs) | Pattern c_1 vs_1 <- merge ms_1 m, c_1 == c]




\h{#mp}\begin{code}
sat $ Sat (Value c xs) [merge ms_1 m :* ms_2] ==>
    sat $ Sat (Value c xs) [ms_1 :* ms_2]
    -- inline |sat|
sat' $ (c <| [merge ms_1 m :* ms_2]) /# ([0..],xs) ==> sat' $ (c <| [ms_1 :* ms_2]) /# ([0..],xs)
    -- inline | <|| |
sat' $ propOrs (map f [merge ms_1 m :* ms_2]) /# ([0..],xs) ==> sat' $ propOrs (map f [ms_1 :* ms_2]) /# ([0..],xs)
    -- inline |map|
sat' $ propOrs [f $ merge ms_1 m :* ms_2] /# ([0..],xs) ==> sat' $ propOrs [f $ ms_1 :* ms_2] /# ([0..],xs)
    -- inline |propOrs|
sat' $ (f $ merge ms_1 m :* ms_2) /# ([0..],xs) ==> sat' $ (f $ ms_1 :* ms_2) /# ([0..],xs)
    -- inline |f|
sat' $ orP [andP $ map lit $ g vs_1 | Pattern c_1 vs_1 <- merge ms_1 m, c_1 == c] /# ([0..],xs) ==> sat' $ (f $ ms_1 :* ms_2) /# ([0..],xs)


sat (Sat (Value c xs)  k) = sat' $ (c <| k) /# ([0..],xs)


\end{code}


\todo{prove merge1}

\begin{comment}
\h{#mp exprlist}\begin{code}
sat $ Sat (Value c xs) [merge ms_1 ms_2 :* merge ms_1 ms_2] ==> sat $ Sat (Value c xs) [ms_1 :* ms_2]
    -- inline |sat|
sat' $ (c <| [merge ms_1 ms_2 :* merge ms_1 ms_2]) /# ([0..],xs) ==> sat' $ (c <| [ms_1 :* ms_2]) /# ([0..],xs)
    -- inline | <|| |
sat' $ propOrs (map f [merge ms_1 ms_2 :* merge ms_1 ms_2]) /# ([0..],xs) ==> sat' $ propOrs (map f [ms_1 :* ms_2]) /# ([0..],xs)
    -- inline |map|
sat' $ propOrs [f $ merge ms_1 ms_2 :* merge ms_1 ms_2] /# ([0..],xs) ==> sat' $ propOrs [f $ ms_1 :* ms_2] /# ([0..],xs)
    -- inline |propOrs|
sat' $ (f $ merge ms_1 ms_2 :* merge ms_1 ms_2) /# ([0..],xs) ==> sat' $ (f $ ms_1 :* ms_2) /# ([0..],xs)
    -- inline |f|
sat' $ propOrs [propAnds $ map propLit $ g vs_1 | Pattern c_1 vs_1 <- merge ms_1 ms_2, c_1 == c] /# ([0..],xs) ==> rhs
    -- \todo{finish proof, and change initial theorem}
\end{code}
\end{comment}

\proof{sat/merge2}

\todo{prove merge2}


\proof{sat/|-<|}

\h{#mp exprlist}\begin{code}
sat' (Value c xs -< cs) ==> c `elem` cs
    -- inline |(-<)|
sat' $ propLit $ Sat (Value c xs)
    [map complete cs :* map complete (ctors (head cs)) | not (null cs)] ==> c `elem` cs
\end{code}

Case analysis on |cs|, being either null, or not.

\h{#mp exprlist}\begin{code}
sat' $ propLit $ Sat (Value c xs)
    [map complete cs :* map complete (ctors (head cs)) | not (null cs)] ==> c `elem` cs
    -- |cs == []|
sat' $ propLit $ Sat (Value c xs)
    [map complete [] :* map complete (ctors (head [])) | not (null [])] ==> c `elem` []
    -- inline |null|
sat' $ propLit $ Sat (Value c xs)
    [map complete [] :* map complete (ctors (head [])) | not True] ==> c `elem` []
    -- inline |not|
sat' $ propLit $ Sat (Value c xs)
    [map complete [] :* map complete (ctors (head [])) | False] ==> c `elem` []
    -- reduce list comprehension
sat' $ propLit $ Sat (Value c xs) [] ==> c `elem` []
    -- inline |elem|
sat' $ propLit $ Sat (Value c xs) [] ==> False
    -- inline |sat'|
sat $ Sat (Value c xs) [] ==> False
    -- \lemma{sat/any}
any (\k -> sat $ Sat (Value c xs) [k]) [] ==> False
    -- inline |any|
False ==> False
    -- equal
True
\end{code}

\h{#mp exprlist}\begin{code}
sat' $ propLit $ Sat (Value c xs)
    [map complete cs :* map complete (ctors (head cs)) | not (null cs)] ==> c `elem` cs
    -- |null cs == False|
sat' $ propLit $ Sat (Value c xs)
    [map complete cs :* map complete (ctors (head cs)) | not False] ==> c `elem` cs
    -- inline |not|
sat' $ propLit $ Sat (Value c xs)
    [map complete cs :* map complete (ctors (head cs)) | True] ==> c `elem` cs
    -- simplify list comprehension
sat' $ propLit $ Sat (Value c xs)
    [map complete cs :* map complete (ctors (head cs))] ==> c `elem` cs
    -- inline |sat'|
sat $ Sat (Value c xs)
    [map complete cs :* map complete (ctors (head cs))] ==> c `elem` cs
    -- inline |sat|
sat' $ (c <| [map complete cs :* map complete (ctors (head cs))])
    /# ([0..],xs) ==> c `elem` cs
    -- inline | <|| |
sat' $ (propOrs $ map f [map complete cs :* map complete (ctors (head cs))])
    /# ([0..],xs) ==> c `elem` cs
    -- inline |map|
sat' $ (propOrs [f $ map complete cs :* map complete (ctors (head cs))])
    /# ([0..],xs) ==> c `elem` cs
    -- inline |propOr|
sat' $ (f $ map complete cs :* map complete (ctors (head cs)))
    /# ([0..],xs) ==> c `elem` cs
    -- inline |f|
sat' $ propOrs [propAnds $ map propLit $ g vs_1 | Pattern c_1 vs_1 <- map complete cs, c_1 == c]
    /# ([0..],xs) ==> c `elem` cs
    -- inline |(/)|
sat' $ propOrs [propAnds $ map propLit $ g vs_1 /# ([0..],xs) |
    Pattern c_1 vs_1 <- map complete cs, c_1 == c] ==> c `elem` cs
    -- inline |sat'|
or [sat' $ propAnds $ map propLit $ g vs_1 /# ([0..],xs) |
    Pattern c_1 vs_1 <- map complete cs, c_1 == c] ==> c `elem` cs
    -- move the guard
or [c_1 == c && sat' (propAnds $ map propLit $ g vs_1 /# ([0..],xs)) |
    Pattern c_1 vs_1 <- map complete cs] ==> c `elem` cs
    -- remove the list comprehension
any (\(Pattern c_1 vs_1) -> c_1 == c &&
    sat' (propAnds $ map propLit $ g vs_1 /# ([0..],xs))) (map complete cs) ==> c `elem` cs
    -- |any f (map g xs) = any (f . g) xs|
any ((\(Pattern c_1 vs_1) -> c_1 == c &&
    sat' (propAnds $ map propLit $ g vs_1 /# ([0..],xs))) . complete) cs ==> c `elem` cs
    -- |c `elem` cs == any (== c) cs|
any ((\(Pattern c_1 vs_1) -> c_1 == c &&
    sat' (propAnds $ map propLit $ g vs_1 /# ([0..],xs))) . complete) cs ==> any (== c) cs
    -- lift implication over |any|
(\(Pattern c_1 vs_1) -> c_1 == c &&
    sat' (propAnds $ map propLit $ g vs_1 /# ([0..],xs))) (complete c') ==> c' == c
    -- inline |complete|
c' == c && sat' (propAnds $ map propLit $ g (map (const Any) (nonRecs c'))
    /# ([0..],xs)) ==> c' == c
    -- weaken implication
c' == c ==> c' == c
    -- equals
True
\end{code}

\proof{sat/| ||> |}

\h{#mp exprlist}\begin{code}
sat $ Sat (Value c xs) ((c,i) |> k) ==> sat $ Sat (xs !! i) k
    -- inline | ||> |
sat $ Sat (Value c xs) (map f k) ==> sat $ Sat (xs !! i) k
    -- inline |sat|
sat' $ (c <| map f_rhd k) /# ([0..],xs) ==> sat $ Sat (xs !! i) k
    -- inline | <|| |
sat' $ propOrs (map f_lhd (map f_rhd k)) /# ([0..],xs) ==> sat $ Sat (xs !! i) k
    -- |map f . map g = map (f . g)|
sat' $ propOrs (map (f_lhd . f_rhd) k) /# ([0..],xs) ==> sat $ Sat (xs !! i) k
\end{code}

We now proceed by induction over |k|. We assume |k| may take the values |[]|, |Any:ks| and \h{#mp}|(ms_1 :* ms_2):ks|.

\proof[|[]|]{sat/| ||> |}

\h{#mp exprlist}\begin{code}
sat' $ propOrs (map (f_lhd . f_rhd) k) /# ([0..],xs) ==> sat $ Sat (xs !! i) k
    -- |k == []|
sat' $ propOrs (map (f_lhd . f_rhd) []) /# ([0..],xs) ==> sat $ Sat (xs !! i) []
    -- inline |map|
sat' $ propOrs [] /# ([0..],xs) ==> sat $ Sat (xs !! i) []
    -- inline |propOrs|
sat' $ propFalse /# ([0..],xs) ==> sat $ Sat (xs !! i) []
    -- inline |(/)|
sat' propFalse ==> sat $ Sat (xs !! i) []
    -- inline |sat'|
False ==> sat $ Sat (xs !! i) []
    -- implication
True
\end{code}

\proof[|Any:ks|]{sat/| ||> |}

\h{#mp exprlist}\begin{code}
sat' $ propOrs (map (f_lhd . f_rhd) k) /# ([0..],xs) ==> sat $ Sat (xs !! i) k
    -- |k == Any:ks|
sat' $ propOrs (map (f_lhd . f_rhd) (Any:ks)) /# ([0..],xs) ==> sat $ Sat (xs !! i) (Any:ks)
    -- weaken implication
sat $ Sat (xs !! i) (Any:ks)
\end{code}

Now, by case analysis on |xs !! i|, first assuming |xs !! i == Bottom|, then |Value c xs|.

\h{#mp exprlist}\begin{code}
sat $ Sat (xs !! i) (Any:ks)
    -- |xs !! i == Bottom|
sat $ Sat Bottom (Any:ks)
    -- inline |sat|
True
\end{code}

\h{#mp exprlist}\begin{code}
sat $ Sat (xs !! i) (Any:ks)
    -- |xs !! i == Value c xs|
sat $ Sat (Value c xs) (Any:ks)
    -- inline |sat|
sat' $ (c <| (Any:ks)) /# ([0..],xs)
    -- inline | <|| |
sat' $ propOrs (map f (Any:ks)) /# ([0..],xs)
    -- inline |map f|
sat' $ propOrs (propTrue : map f ks) /# ([0..],xs)
    -- inline |propOrs|
sat' $ propTrue /# ([0..],xs)
    -- inline |(/)|
sat' propTrue
    -- inline |sat'|
True
\end{code}

\proof[\ignore|(ms_1 :* ms_2):ks|]{sat/| ||> |}

\h{#mp exprlist}\begin{code}
sat' $ propOrs (map (f_lhd . f_rhd) k) /# ([0..],xs) ==> sat $ Sat (xs !! i) k
    -- |k == (ms_1 :* ms_2):ks|
sat' $ propOrs (map (f_lhd . f_rhd) ((ms_1 :* ms_2):ks)) /# ([0..],xs) ==>
    sat $ Sat (xs !! i) ((ms_1 :* ms_2):ks)
    -- inline |map|
sat' $ propOrs ((f_lhd $ f_rhd $ ms_1 :* ms_2) : map (f_lhd . f_rhd) ks) /# ([0..],xs) ==> rhs
    -- inline |(/)|
sat' $ propOrs (((f_lhd $ f_rhd $ ms_1 :* ms_2) /# ([0..],xs)) :
    (map (f_lhd . f_rhd) ks /# ([0..],xs))) ==> rhs
    -- inline |propOrs|
sat' $ ((f_lhd $ f_rhd $ ms_1 :* ms_2) /# ([0..],xs)) `propOr`
    propOrs (map (f_lhd . f_rhd) ks /# ([0..],xs)) ==> rhs
    -- inline |sat'|
sat' ((f_lhd $ f_rhd $ ms_1 :* ms_2) /# ([0..],xs)) ||
    sat' (propOrs (map (f_lhd . f_rhd) ks /# ([0..],xs))) ==> rhs
    -- reinstate RHS
sat' ((f_lhd $ f_rhd $ ms_1 :* ms_2) /# ([0..],xs)) ||
    sat' (propOrs (map (f_lhd . f_rhd) ks /# ([0..],xs))) ==>
    sat $ Sat (xs !! i) ((ms_1 :* ms_2):ks)
\end{code}

Now by case analysis. Either |xs !! i == Bottom|, or |Value c' ys|

\h{#mp exprlist}\begin{code}
sat' ((f_lhd $ f_rhd $ ms_1 :* ms_2) /# ([0..],xs)) ||
    sat' (propOrs (map (f_lhd . f_rhd) ks /# ([0..],xs))) ==>
    sat $ Sat (xs !! i) ((ms_1 :* ms_2):ks)
    -- weaken implication
sat $ Sat (xs !! i) ((ms_1 :* ms_2):ks)
    -- |xs !! i = Bottom|
sat $ Sat Bottom ((ms_1 :* ms_2):ks)
    -- inline |sat|
True
\end{code}

\h{#mp exprlist}\begin{code}
sat' ((f_lhd $ f_rhd $ ms_1 :* ms_2) /# ([0..],xs)) ||
    sat' (propOrs (map (f_lhd . f_rhd) ks /# ([0..],xs))) ==>
    sat $ Sat (xs !! i) ((ms_1 :* ms_2):ks)
    -- |xs !! i = Value c' ys|
lhs ==> sat $ Sat (Value c' ys) ((ms_1 :* ms_2):ks)
    -- \lemma{sat/any}
lhs ==> any (\k -> sat $ Sat (Value c' ys) [k]) ((ms_1 :* ms_2):ks)
    -- inline |any|
lhs ==> sat (Sat (Value c' ys) [ms_1 :* ms_2]) ||
    any (\k -> sat $ Sat (Value c' xs) [k]) ks
    -- \lemma{sat/any}
lhs ==> sat (Sat (Value c' ys) [ms_1 :* ms_2]) || sat (Sat (Value c' ys) ks)
    -- reinstate LHS
sat' ((f_lhd $ f_rhd $ ms_1 :* ms_2) /# ([0..],xs)) ||
    sat' (propOrs (map (f_lhd . f_rhd) ks /# ([0..],xs))) ==>
    sat (Sat (Value c ys) [ms_1 :* ms_2]) || sat (Sat (Value c' ys) ks)
    -- split the implication
(sat' ((f_lhd $ f_rhd $ ms_1 :* ms_2) /# ([0..],xs)) ==>
    sat (Sat (Value c' ys) [ms_1 :* ms_2])) &&
    (sat' (propOrs (map (f_lhd . f_rhd) ks /# ([0..],xs))) ==> sat (Sat (Value c' ys) ks))
    -- |xs !! i == Value c' ys|
(sat' ((f_lhd $ f_rhd $ ms_1 :* ms_2) /# ([0..],xs)) ==> sat (Sat (xs !! i) [ms_1 :* ms_2])) &&
    (sat' (propOrs (map (f_lhd . f_rhd) ks /# ([0..],xs))) ==> sat (Sat (xs !! i) ks))
    -- inductive hypothesis
sat' $ (f_lhd $ f_rhd $ ms_1 :* ms_2) /# ([0..],xs) ==>
    sat $ Sat (xs !! i) [ms_1 :* ms_2]
\end{code}

We can now perform case analysis, assuming either |isRec (c,i) == False|, or the reverse.

\h{#mp exprlist}\begin{code}
sat' $ (f_lhd $ f_rhd $ ms_1 :* ms_2) /# ([0..],xs) ==> sat $ Sat (xs !! i) [ms_1 :* ms_2]
    -- inline |f_rhd|, assuming |isRec (c,i) == False|
sat' $ (f_lhd $ [Pattern c [if i == j then ms_1 :* ms_2 else Any | j <- nonRecs c]] :*
    map complete (ctors c)) /# ([0..],xs) ==> lhs
    -- inline |f_lhd|
sat' $ propOrs [propAnds $ map propLit $ g vs_1 | Pattern c_1 vs_1 <-
    [Pattern c [if i == j then ms_1 :* ms_2 else Any | j <- nonRecs c]],
     c_1 == c] /# ([0..],xs) ==> lhs
    -- simplify list comprehension
sat' $ propOrs [propAnds $ map propLit $ g
    [if i == j then ms_1 :* ms_2 else Any | j <- nonRecs c]]
    /# ([0..],xs) ==> lhs
    -- inline |propOrs|
sat' $ (propAnds $ map propLit $ g
    [if i == j then ms_1 :* ms_2 else Any | j <- nonRecs c])
    /# ([0..],xs) ==> lhs
    -- inline |(/)|
sat' $ propAnds $ map propLit $ g
    [if i == j then ms_1 :* ms_2 else Any | j <- nonRecs c]
    /# ([0..],xs) ==> lhs
    -- inline |sat'|
all sat $ g [if i == j then ms_1 :* ms_2 else Any | j <- nonRecs c]
    /# ([0..],xs) ==> lhs
    -- inline |g|
all sat $ (zipWith Sat non (map (:[])
    [if i == j then ms_1 :* ms_2 else Any | j <- nonRecs c]) ++
    map (`Sat` [map complete (ctors c) :* map complete (ctors c)]) rec)
    /# ([0..],xs) ==> lhs
    -- inline |(/)|
all sat $ zipWith Sat (non /# ([0..],xs))
    (map (:[]) [if i == j then ms_1 :* ms_2 else Any | j <- nonRecs c]) ++
    map (`Sat` [map complete (ctors c) :* map complete (ctors c)])
    (rec /# ([0..],xs)) ==> lhs
    -- inline |all|
all sat (zipWith Sat (non /# ([0..],xs))
    (map (:[]) [if i == j then ms_1 :* ms_2 else Any | j <- nonRecs c])) &&
    all sat (map (`Sat` [map complete (ctors c) :* map complete (ctors c)])
    (rec /# ([0..],xs))) ==> lhs
    -- weaken implication
all sat $ zipWith Sat (non /# ([0..],xs))
    (map (:[]) [if i == j then ms_1 :* ms_2 else Any | j <- nonRecs c]) ==> lhs
    -- inline |map|
all sat $ zipWith Sat (non /# ([0..],xs))
    [if i == j then [ms_1 :* ms_2] else [Any] | j <- nonRecs c] ==> lhs
    -- |non == nonRecs c|, by definition of |nonRecs|
all sat $ zipWith Sat (non /# ([0..],xs))
    [if i == j then [ms_1 :* ms_2] else [Any] | j <- non] ==> lhs
    -- rewrite list comprehension
all sat $ zipWith Sat (non /# ([0..],xs))
    (map (\j -> if i == j then [ms_1 :* ms_2] else [Any]) non) ==> lhs
    -- inline |(/)|
all sat $ zipWith Sat (map (/# ([0..],xs)) non)
    (map (\j -> if i == j then [ms_1 :* ms_2] else [Any]) non) ==> lhs
    -- |zipWith f (map g xs) (map h xs) == map (\x -> f (g x) (h x)) xs|
all sat $ map (\j -> Sat (j /# ([0..],xs))
    (if i == j then [ms_1 :* ms_2] else [Any])) non ==> lhs
    -- weaken implication, using |i `elem` non| because of false |isRec| test
all sat $ map (\j -> Sat (j /# ([0..],xs))
    (if i == j then [ms_1 :* ms_2] else [Any])) [i] ==> lhs
    -- inline |map|
all sat $ [Sat (i /# ([0..],xs)) (if i == i then [ms_1 :* ms_2] else [Any])] ==> lhs
    -- inline |all|
sat $ Sat (i /# ([0..],xs)) (if i == i then [ms_1 :* ms_2] else [Any]) ==> lhs
    -- |(i == i) == True|
sat $ Sat (i /# ([0..],xs)) [ms_1 :* ms_2] ==> lhs
    -- inline |(/)|
sat $ Sat (xs !! i) [ms_1 :* ms_2] ==> lhs
    -- reinstate LHS
sat $ Sat (xs !! i) [ms_1 :* ms_2] ==> sat $ Sat (xs !! i) [ms_1 :* ms_2]
    -- equals
True
\end{code}


\h{#mp exprlist}\begin{code}
sat' $ (f_lhd $ f_rhd $ ms_1 :* ms_2) /# ([0..],xs) ==> sat $ Sat (xs !! i) [ms_1 :* ms_2]
    -- inline |f_rhd|, assuming |isRec (c,i)|
sat' $ (f_lhd $ [complete c] :* merge ms_1 ms_2) /# ([0..],xs) ==> lhs
    -- inline |f_lhd|
sat' $ propOrs [propAnds $ map propLit $ g vs_1 |
    Pattern c_1 vs_1 <- [complete c], c_1 == c] /# ([0..],xs) ==> lhs
    -- inline |complete c|
sat' $ propOrs [propAnds $ map propLit $ g vs_1 | Pattern c_1 vs_1 <-
    [Pattern c (map (const Any) (nonRecs c))], c_1 == c] /# ([0..],xs) ==> lhs
    -- simplify list comprehension
sat' $ propOrs [propAnds $ map propLit $ g $ map (const Any) (nonRecs c)]
    /# ([0..],xs) ==> lhs
    -- inline |propOrs|
sat' $ propAnds (map propLit $ g $ map (const Any) (nonRecs c))
    /# ([0..],xs) ==> lhs
    -- inline |(/)|
sat' $ propAnds $ map propLit $ (g $ map (const Any) (nonRecs c))
    /# ([0..],xs) ==> lhs
    -- inline |sat'|
all sat $ (g $ map (const Any) (nonRecs c)) /# ([0..],xs) ==> lhs
    -- inline |g|
all sat $ (zipWith Sat non (map (:[]) vs) ++
    map (`Sat` [merge ms_1 ms_2 :* merge ms_1 ms_2]) rec) /# ([0..],xs) ==> lhs
    -- inline |(/)|
all sat $ zipWith Sat non (map (:[]) vs) /# ([0..],xs) ++
    map (`Sat` [merge ms_1 ms_2 :* merge ms_1 ms_2]) rec /# ([0..],xs) ==> lhs
    -- inline |all|
all sat (zipWith Sat non (map (:[]) vs) /# ([0..],xs)) &&
    all sat (map (`Sat` [merge ms_1 ms_2 :* merge ms_1 ms_2]) rec
    /# ([0..],xs)) ==> lhs
    -- weaken implication
all sat $ map (`Sat` [merge ms_1 ms_2 :* merge ms_1 ms_2]) rec
    /# ([0..],xs) ==> lhs
    -- eta expand
all sat $ map (\j -> Sat j [merge ms_1 ms_2 :* merge ms_1 ms_2]) rec
    /# ([0..],xs) ==> lhs
    -- inline |(/)|
all sat $ map (\j -> Sat (j /# ([0..],xs))
    [merge ms_1 ms_2 :* merge ms_1 ms_2]) rec ==> lhs
    -- combine |all| and |map|
all (\j -> sat $ Sat (j /# ([0..],xs))
    [merge ms_1 ms_2 :* merge ms_1 ms_2]) rec ==> lhs
    -- weaken implication, as |i `elem` rec|, because of |isRec| test
all (\j -> sat $ Sat (j /# ([0..],xs))
    [merge ms_1 ms_2 :* merge ms_1 ms_2]) [i] ==> lhs
    -- inline |all|
sat $ Sat (i /# ([0..],xs)) [merge ms_1 ms_2 :* merge ms_1 ms_2] ==> lhs
    -- inline |(/)|
sat $ Sat (xs !! i) [merge ms_1 ms_2 :* merge ms_1 ms_2] ==> rhs
    -- reinstate RHS
sat $ Sat (xs !! i) [merge ms_1 ms_2 :* merge ms_1 ms_2] ==>
    sat $ Sat (xs !! i) [ms_1 :* ms_2]
    -- |xs !! i == Value c' ys|
sat $ Sat (Value c' ys) [merge ms_1 ms_2 :* merge ms_1 ms_2] ==>
    sat $ Sat (Value c' ys) [ms_1 :* ms_2]
    -- \lemma{sat/merge1}
sat $ Sat (Value c' ys) [ms_1 :* merge ms_1 ms_2] ==>
    sat $ Sat (Value c' ys) [ms_1 :* ms_2]
    -- \lemma{sat/merge2}
sat $ Sat (Value c' ys) [ms_1 :* ms_2] ==> sat $ Sat (Value c' ys) [ms_1 :* ms_2]
    -- equal
True
\end{code}

